Update TreapNode.dfy

TreapNode.dfy
@@ -3,7 +3,6 @@ class TreapNode {
   const priority: int
   var left: TreapNode?
   var right: TreapNode?
-  var parent: TreapNode?
 
   // Needed to ensure no cycles in between nodes
   ghost var repr: set<TreapNode>
@@ -11,29 +10,38 @@ class TreapNode {
   ghost predicate Valid()
     reads this, repr
   {
-    && this in repr
+    && this in repr // node is reachable to itself
     && ( left != null ==>
          && left in repr
          && this !in left.repr
-         && left.repr <= repr
+         && left.repr < repr
          && left.Valid())
     && ( right != null ==>
          && right in repr
          && this !in right.repr
-         && right.repr <= repr
+         && right.repr < repr
          && right.Valid())
     && ( // Extra check to ensure only one path between 2 nodes.
-       right != null && right.Valid() && left != null && left.Valid() ==>
-         (forall x :: x in left.repr ==> x !in right.repr) &&
-         (forall y :: y in right.repr ==> y !in left.repr))
+       (right != null && left != null) ==>
+         ((forall x :: x in left.repr ==> x !in right.repr) &&
+                       (forall y :: y in right.repr ==> y !in left.repr)))
   }
 
-  constructor (key:int, priority:int) {
+  predicate IsLeaf()
+    reads this
+  {
+    && this.left == null
+    && this.right == null
+  }
+
+  constructor (key:int, priority:int)
+    ensures Valid()
+    ensures repr == {this}
+  {
     this.key := key;
     this.priority := priority;
     this.left := null;
     this.right := null;
-    this.parent := null;
     repr := {this};
   }
 }
